SoLean.lean
@@ -7,6 +7,7 @@ import SoLean.Examples.CounterYul
 import SoLean.Examples.AAWallet
 import SoLean.Examples.AAPQIntegration
 import SoLean.Examples.AAPQEvmCall
+import SoLean.Examples.AAPQEvmCallGas
 import SoLean.Examples.AAPQSource
 import SoLean.Examples.PQVerifierWrapper
 import SoLean.Examples.ToyVerifier
